src/cddl/spec/CDDL.Spec.Base.fst
@@ -228,3 +228,19 @@ let spec_choice
   serializer = serializer_spec_choice p1.serializer p2.serializer _;
   parser_inj = ();
 }
+
+let parser_spec_always_false (p: squash False -> bool) : parser_spec t_always_false (squash False) p =
+  (fun x -> false_elim ())
+
+let serializer_spec_always_false (p: squash False -> bool) : serializer_spec (parser_spec_always_false p) =
+  (fun x -> false_elim ())
+
+let spec_always_false
+  (p: (squash False -> bool))
+: spec t_always_false (squash False) true
+= {
+  serializable = p;
+  parser = parser_spec_always_false p;
+  serializer = serializer_spec_always_false p;
+  parser_inj = ();
+}
